src/Examples/HACMSDemo/HACMSDemo.v
@@ -1,0 +1,433 @@
+Require Import Coq.Strings.Ascii
+        Coq.Bool.Bool
+        Coq.Lists.List
+        Coq.Structures.OrderedType.
+
+Require Import
+        Fiat.BinEncoders.Env.BinLib.Core
+        Fiat.BinEncoders.Env.Common.Specs
+        Fiat.BinEncoders.Env.Common.Compose
+        Fiat.BinEncoders.Env.Common.ComposeOpt
+        Fiat.BinEncoders.Env.Automation.Solver
+        Fiat.BinEncoders.Env.Lib2.WordOpt
+        Fiat.BinEncoders.Env.Lib2.NatOpt
+        Fiat.BinEncoders.Env.Lib2.StringOpt
+        Fiat.BinEncoders.Env.Lib2.EnumOpt
+        Fiat.BinEncoders.Env.Lib2.FixListOpt
+        Fiat.BinEncoders.Env.Lib2.SumTypeOpt.
+
+Require Import
+        Fiat.Common.SumType
+        Fiat.Examples.Tutorial.Tutorial
+        Fiat.Examples.DnsServer.DecomposeEnumField
+        Fiat.QueryStructure.Automation.AutoDB
+        Fiat.QueryStructure.Implementation.DataStructures.BagADT.BagADT
+        Fiat.QueryStructure.Automation.IndexSelection
+        Fiat.QueryStructure.Specification.SearchTerms.ListPrefix
+        Fiat.QueryStructure.Automation.SearchTerms.FindPrefixSearchTerms
+        Fiat.Examples.HACMSDemo.DuplicateFree
+        Fiat.QueryStructure.Automation.MasterPlan.
+
+Require Import
+        Bedrock.Word
+        Bedrock.Memory.
+
+Lemma exists_CompletelyUnConstrFreshIdx:
+  forall (qs_schema : RawQueryStructureSchema)
+    (BagIndexKeys : ilist3 (qschemaSchemas qs_schema))
+    (r_o : UnConstrQueryStructure qs_schema)
+    (r_n : IndexedQueryStructure qs_schema BagIndexKeys),
+  DelegateToBag_AbsR r_o r_n ->
+  exists bnd : nat,
+  forall idx : Fin.t (numRawQSschemaSchemas qs_schema),
+    UnConstrFreshIdx (GetUnConstrRelation r_o idx) bnd.
+Proof.
+  intros.
+  generalize (exists_UnConstrFreshIdx H); clear H.
+  remember (GetUnConstrRelation r_o); clear.
+  destruct qs_schema; simpl in *.
+  clear qschemaConstraints.
+  induction numRawQSschemaSchemas; simpl in *; intros.
+  - exists 0; intros; inversion idx.
+  - revert i IHnumRawQSschemaSchemas H.
+    pattern numRawQSschemaSchemas, qschemaSchemas;
+      apply Vector.caseS; simpl; intros.
+    destruct (IHnumRawQSschemaSchemas
+                t
+                (fun idx => i (Fin.FS idx))
+                (fun idx => H (Fin.FS idx))
+             ).
+    destruct (H Fin.F1).
+    exists (max x x0).
+    unfold UnConstrFreshIdx in *; simpl in *; intros.
+    pose proof (Max.le_max_l x x0);
+      pose proof (Max.le_max_r x x0).
+    generalize dependent idx; intro; generalize t i x x0 H0 H1 H3 H4;
+      clear; pattern n, idx; apply Fin.caseS; simpl; intros.
+    apply H1 in H2; omega.
+    apply H0 in H2; omega.
+Qed.
+
+Lemma refine_Pick_CompletelyUnConstrFreshIdx
+  : forall (qs_schema : RawQueryStructureSchema)
+    (BagIndexKeys : ilist3 (qschemaSchemas qs_schema))
+    (r_o : UnConstrQueryStructure qs_schema)
+    (r_n : IndexedQueryStructure qs_schema BagIndexKeys),
+    DelegateToBag_AbsR r_o r_n ->
+    forall (bnd : nat),
+      (forall (idx : Fin.t (numRawQSschemaSchemas qs_schema)),
+          UnConstrFreshIdx (GetUnConstrRelation r_o idx) bnd) ->
+      refine {bnd0 : nat | forall idx, UnConstrFreshIdx (GetUnConstrRelation r_o idx) bnd0} (ret bnd).
+Proof.
+  intros; refine pick val _; eauto.
+  reflexivity.
+Qed.
+
+Instance Query_eq_word32 : Query_eq (word 32) :=
+  {| A_eq_dec := @weq 32 |}.
+
+Global Instance GetAttributeRawTermCounter' {A : Type} {qsSchema}
+         {Ridx : Fin.t _}
+         {tup : @RawTuple (Vector.nth _ Ridx)}
+         {BAidx : _ }
+         a
+    : (TermAttributeCounter qsSchema (@GetAttributeRaw {| NumAttr := S _;
+                                                          AttrList := Vector.cons _ A _ _ |} {|prim_fst := a; prim_snd := tup |} (Fin.FS BAidx)) Ridx BAidx) | 0 := Build_TermAttributeCounter qsSchema _ Ridx BAidx.
+
+Ltac GetAttributeRawTermCounterTac t ::=
+     lazymatch goal with
+       _ =>
+       match goal with
+         |- TermAttributeCounter
+              ?qs_schema
+              (GetAttributeRaw {| prim_fst := ?a;
+                             prim_snd := ?tup |} (Fin.FS ?BAidx))
+         _ _ =>
+    match type of tup with
+    | @RawTuple (@GetNRelSchemaHeading _ _ ?Ridx) =>
+      apply (@GetAttributeRawTermCounter' _ qs_schema Ridx tup _ a)
+    end
+    end
+  end.
+
+Lemma refineEquiv_Query_Where_And
+      {ResultT}
+  : forall P P' bod,
+    (P \/ ~ P)
+    -> refineEquiv (@Query_Where ResultT (P /\ P') bod)
+                (Query_Where P (Query_Where P' bod)).
+Proof.
+  split; unfold refine, Query_Where; intros;
+    computes_to_inv; computes_to_econstructor;
+      intuition.
+  - computes_to_inv; intuition.
+  - computes_to_inv; intuition.
+  - computes_to_econstructor; intuition.
+Qed.
+
+Corollary refineEquiv_For_Query_Where_And
+          {ResultT}
+          {qs_schema}
+  : forall (r : UnConstrQueryStructure qs_schema) idx P P' bod,
+    (forall tup, P tup \/ ~ P tup)
+    -> refine (For (UnConstrQuery_In
+                      r idx
+                      (fun tup => @Query_Where ResultT (P tup /\ P' tup) (bod tup))))
+              (For (UnConstrQuery_In
+                      r idx
+                      (fun tup => Where (P tup) (Where (P' tup) (bod tup))))).
+Proof.
+  intros; apply refine_refine_For_Proper.
+  apply refine_UnConstrQuery_In_Proper.
+  intro; apply refineEquiv_Query_Where_And; eauto.
+Qed.
+
+Lemma refine_If_IfOpt {A B}
+  : forall (a_opt : option A) (t e : Comp B),
+    refine (If_Then_Else (If_Opt_Then_Else a_opt (fun _ => false) true)
+                         t e)
+           (If_Opt_Then_Else a_opt (fun _ => e) t).
+Proof.
+  destruct a_opt; simpl; intros; reflexivity.
+Qed.
+
+Global Arguments icons2 _ _ _ _ _ _ _ / .
+Global Arguments GetAttributeRaw {heading} !tup !attr .
+Global Arguments ilist2_tl _ _ _ _ !il / .
+Global Arguments ilist2_hd _ _ _ _ !il / .
+
+Global Opaque If_Opt_Then_Else.
+Ltac implement_DecomposeRawQueryStructure :=
+  first [ simplify with monad laws; simpl
+        | rewrite refine_If_IfOpt
+        | match goal with
+            |- refine (b <- If_Opt_Then_Else _ _ _; _) _ =>
+            etransitivity;
+            [ apply refine_If_Opt_Then_Else_Bind
+            | simpl; eapply refine_If_Opt_Then_Else_trans;
+              intros; set_refine_evar ]
+          end
+        | match goal with
+            H0 : DecomposeRawQueryStructureSchema_AbsR' _ _ _ _ ?r_o ?r_n |- refine _ ?H => unfold H;
+                                                                                            apply (refine_UnConstrFreshIdx_DecomposeRawQueryStructureSchema_AbsR_Equiv H0 Fin.F1)
+          end
+        | match goal with
+            H0 : DecomposeRawQueryStructureSchema_AbsR' (qs_schema := ?qs_schema) _ _ _ _ ?r_o ?r_n |- refine (Query_For _ ) _ =>
+            rewrite (refineEquiv_For_Query_Where_And r_o Fin.F1); eauto
+          end
+        |
+        match goal with
+          H0 : DecomposeRawQueryStructureSchema_AbsR' (qs_schema := ?qs_schema) _ _ _ _ ?r_o ?r_n |- refine (Query_For _ ) _ =>
+          rewrite (@refine_QueryIn_Where _ qs_schema Fin.F1 _ _ _ _ _ H0 _ _ _ );
+          unfold Tuple_DecomposeRawQueryStructure_inj; simpl
+        end
+        | match goal with
+            H0 : DecomposeRawQueryStructureSchema_AbsR' _ _ _ _ ?r_o ?r_n
+            |- refine { r_n | DecomposeRawQueryStructureSchema_AbsR' _ _ _ _ _ r_n} _ =>
+            first [refine pick val _; [ | eassumption ]
+                  | refine pick val _;
+                    [ | apply (DecomposeRawQueryStructureSchema_Insert_AbsR_eq H0) ] ]
+          end
+        ].
+
+Ltac implement_DecomposeRawQueryStructure' H :=
+  first [
+      simplify with monad laws; simpl
+    | rewrite H
+    | apply refine_pick_eq'
+    | etransitivity;
+      [ apply refine_If_Opt_Then_Else_Bind
+      | simpl; eapply refine_If_Opt_Then_Else_trans;
+        intros; set_refine_evar ] ].
+
+  Lemma GetAttributeRaw_FS
+    : forall {A} {heading} (a : A) (tup : @RawTuple heading) n,
+      @GetAttributeRaw {| AttrList := Vector.cons _ A _ (AttrList heading) |}
+                       {| prim_fst := a; prim_snd := tup |} (Fin.FS n)
+    = GetAttributeRaw tup n.
+  Proof.
+    unfold GetAttributeRaw; simpl; reflexivity.
+  Qed.
+
+    Lemma GetAttributeRaw_F1
+    : forall {A} {heading} (a : A) (tup : @RawTuple heading),
+      @GetAttributeRaw {| AttrList := Vector.cons _ A _ (AttrList heading) |}
+                       {| prim_fst := a; prim_snd := tup |} Fin.F1
+    = a.
+  Proof.
+    unfold GetAttributeRaw; simpl; reflexivity.
+  Qed.
+
+  Module word_as_OT <: OrderedType.
+    Definition t := word 32.
+    Definition eq (c1 c2 : t) := c1 = c2.
+    Definition lt (c1 c2 : t) := wlt c1 c2.
+
+    Definition eq_dec : forall l l', {eq l l'} + {~eq l l'} := @weq 32 .
+
+    Lemma eq_refl : forall x, eq x x.
+    Proof. reflexivity. Qed.
+
+    Lemma eq_sym : forall x y, eq x y -> eq y x.
+    Proof. intros. symmetry. eauto. Qed.
+
+    Lemma eq_trans : forall x y z, eq x y -> eq y z -> eq x z.
+    Proof. intros. unfold eq in *. rewrite H. rewrite H0. eauto. Qed.
+
+    Lemma lt_trans : forall x y z, lt x y -> lt y z -> lt x z.
+    Proof. intros. unfold lt in *. eapply N.lt_trans; eauto. Qed.
+
+    Lemma lt_not_eq : forall x y, lt x y -> ~eq x y.
+    Proof.
+      intros. unfold eq, lt, wlt in *. intro.
+      rewrite <- N.compare_lt_iff in H.
+      subst; rewrite N.compare_refl in H; discriminate.
+    Qed.
+
+    Lemma compare : forall x y, Compare lt eq x y.
+    Proof.
+      intros. unfold lt, eq, wlt.
+      destruct (N.compare (wordToN x) (wordToN y)) eqn: eq.
+      - eapply EQ. apply N.compare_eq_iff in eq; apply wordToN_inj; eauto.
+      - eapply LT. abstract (rewrite <- N.compare_lt_iff; eauto).
+      - eapply GT. abstract (rewrite <- N.compare_gt_iff; eauto).
+    Defined.
+End word_as_OT.
+
+Module wordIndexedMap := FMapAVL.Make word_as_OT.
+
+Module wordTreeBag := TreeBag wordIndexedMap.
+
+Ltac BuildQSIndexedBag heading AttrList BuildEarlyBag BuildLastBag k ::=
+  lazymatch AttrList with
+  | (?Attr :: [ ])%list =>
+    let AttrKind := eval simpl in (KindIndexKind Attr) in
+        let AttrIndex := eval simpl in (KindIndexIndex Attr) in
+            let is_equality := eval compute in (string_dec AttrKind "EqualityIndex") in
+
+                lazymatch is_equality with
+                | left _ =>
+                  let AttrType := eval compute in (Domain heading AttrIndex) in
+                      lazymatch AttrType with
+                      | BinNums.N =>
+                        k (@NTreeBag.IndexedBagAsCorrectBag
+                             _ _ _ _ _ _ _
+                             (@CountingListAsCorrectBag
+                                (@RawTuple heading)
+                                (IndexedTreeUpdateTermType heading)
+                                (IndexedTreebupdate_transform heading))
+                             (fun x => GetAttributeRaw (heading := heading) x AttrIndex)
+                          )
+                      | word 32 =>
+                        k (@wordTreeBag.IndexedBagAsCorrectBag
+                             _ _ _ _ _ _ _
+                             (@CountingListAsCorrectBag
+                                (@RawTuple heading)
+                                (IndexedTreeUpdateTermType heading)
+                                (IndexedTreebupdate_transform heading))
+                             (fun x => GetAttributeRaw (heading := heading) x AttrIndex)
+                          )
+
+                      | BinNums.Z =>
+                        k (@ZTreeBag.IndexedBagAsCorrectBag
+                             _ _ _ _ _ _ _
+                             (@CountingListAsCorrectBag
+                                (@RawTuple heading)
+                                (IndexedTreeUpdateTermType heading)
+                                (IndexedTreebupdate_transform heading))
+                             (fun x => GetAttributeRaw (heading := heading) x AttrIndex)
+                          )
+                      | nat =>
+                        k (@NatTreeBag.IndexedBagAsCorrectBag
+                             _ _ _ _ _ _ _
+                             (@CountingListAsCorrectBag
+                                (@RawTuple heading)
+                                (IndexedTreeUpdateTermType heading)
+                                (IndexedTreebupdate_transform heading))
+                             (fun x => GetAttributeRaw (heading := heading) x AttrIndex)
+                          )
+                      | string =>
+                        k (@StringTreeBag.IndexedBagAsCorrectBag
+                             _ _ _ _ _ _ _
+                             (@CountingListAsCorrectBag
+                                (@RawTuple heading)
+                                (IndexedTreeUpdateTermType heading)
+                                (IndexedTreebupdate_transform heading))
+                             (fun x => GetAttributeRaw (heading := heading) x AttrIndex)
+                          )
+                      end
+                | right _ =>
+                  BuildLastBag heading AttrList AttrKind AttrIndex k
+                end
+  | (?Attr :: ?AttrList')%list =>
+    let AttrKind := eval simpl in (KindIndexKind Attr) in
+        let AttrIndex := eval simpl in (KindIndexIndex Attr) in
+            let is_equality := eval compute in (string_dec AttrKind "EqualityIndex") in
+                lazymatch is_equality with
+                | left _ =>
+                  let AttrType := eval compute in (Domain heading AttrIndex) in
+                      lazymatch AttrType with
+                      | BinNums.N =>
+                        BuildQSIndexedBag
+                          heading AttrList'
+                          BuildEarlyBag BuildLastBag
+                          ltac:(fun subtree =>
+                                  k (@NTreeBag.IndexedBagAsCorrectBag
+                                       _ _ _ _ _ _ _ subtree
+                                       (fun x => GetAttributeRaw (heading := heading) x AttrIndex)))
+                      | BinNums.Z =>
+                        BuildQSIndexedBag
+                          heading AttrList'
+                          BuildEarlyBag BuildLastBag
+                          (fun x => GetAttributeRaw x AttrIndex)
+                          ltac:(fun subtree =>
+                                  k (@ZTreeBag.IndexedBagAsCorrectBag
+                                       _ _ _ _ _ _ _ subtree
+                                       (fun x => GetAttributeRaw (heading := heading) x AttrIndex)))
+                      | nat =>
+                        BuildQSIndexedBag
+                          heading AttrList'
+                          BuildEarlyBag BuildLastBag
+                          ltac:(fun subtree =>
+                                  k (@NatTreeBag.IndexedBagAsCorrectBag
+                                       _ _ _ _ _ _ _ subtree
+                                       (fun x => GetAttributeRaw (heading := heading) x AttrIndex)))
+                      | string =>
+                        BuildQSIndexedBag
+                          heading AttrList'
+                          BuildEarlyBag BuildLastBag
+                          ltac:(fun subtree =>
+                                  k (@StringTreeBag.IndexedBagAsCorrectBag
+                                       _ _ _ _ _ _ _ subtree
+                                       (fun x => GetAttributeRaw (heading := heading) x AttrIndex)))
+                      end
+                | right _ =>
+                  BuildQSIndexedBag
+                    heading AttrList'
+                    BuildEarlyBag BuildLastBag
+                    ltac:(fun subtree =>
+                            BuildEarlyBag
+                                 heading AttrList AttrKind AttrIndex subtree k)
+                end
+  | ([ ])%list =>
+    k (@CountingListAsCorrectBag
+         (@RawTuple heading)
+         (IndexedTreeUpdateTermType heading)
+         (IndexedTreebupdate_transform heading))
+  end.
+
+  Ltac rewrite_drill ::=
+       subst_refine_evar; (first
+                             [
+                               match goal with
+                                 |- refine (b <- If_Opt_Then_Else _ _ _; _) _ =>
+                                 etransitivity;
+                                 [ apply refine_If_Opt_Then_Else_Bind
+                                 | simpl; eapply refine_If_Opt_Then_Else_trans;
+                                   intros; set_refine_evar ]
+                               end
+                             | eapply refine_under_bind_both; [ set_refine_evar | intros; set_refine_evar ]
+                             | eapply refine_If_Then_Else; [ set_refine_evar | set_refine_evar ] ] ).
+
+
+  Ltac implement_insert CreateTerm EarlyIndex LastIndex
+       makeClause_dep EarlyIndex_dep LastIndex_dep ::=
+    repeat first
+           [simplify with monad laws; simpl
+           | match goal with
+               |- context [(@GetAttributeRaw ?heading {| prim_fst := ?a;
+                                                         prim_snd := ?tup |} (Fin.FS ?BAidx)) ] =>
+               setoid_rewrite (@GetAttributeRaw_FS
+                                 (Vector.hd (AttrList heading))
+                                 {| AttrList := Vector.tl (AttrList heading)|} a _ BAidx)
+             end
+           | match goal with
+             | |- context [(@GetAttributeRaw ?heading {| prim_fst := ?a;
+                                                         prim_snd := ?tup |} Fin.F1) ] =>
+               rewrite (@GetAttributeRaw_F1
+                          (Vector.hd (AttrList heading))
+                          {| AttrList := Vector.tl (AttrList heading) |} a)
+             end
+           | setoid_rewrite refine_If_Then_Else_Bind
+           | match goal with
+               H : DelegateToBag_AbsR ?r_o ?r_n
+               |- context[Pick (fun idx => forall Ridx, UnConstrFreshIdx (GetUnConstrRelation ?r_o Ridx) idx)] =>
+               let freshIdx := fresh in
+               destruct (exists_CompletelyUnConstrFreshIdx _ _ _ _ H) as [? freshIdx];
+               rewrite (refine_Pick_CompletelyUnConstrFreshIdx _ _ _ _ H _ freshIdx)
+             end
+           | implement_Query CreateTerm EarlyIndex LastIndex
+                             makeClause_dep EarlyIndex_dep LastIndex_dep
+           | progress (rewrite ?refine_BagADT_QSInsert; try setoid_rewrite refine_BagADT_QSInsert); [ | solve [ eauto ] .. ]
+           | progress (rewrite ?refine_Pick_DelegateToBag_AbsR; try setoid_rewrite refine_Pick_DelegateToBag_AbsR); [ | solve [ eauto ] .. ] ].
+
+  Ltac choose_data_structures :=
+    simpl; pose_string_ids; pose_headings_all;
+    pose_search_term;  pose_SearchUpdateTerms;
+    match goal with
+      |- context [ @Build_IndexedQueryStructure_Impl_Sigs _ ?indices ?SearchTerms _ ] => try unfold SearchTerms
+    end; BuildQSIndexedBags' BuildEarlyBag BuildLastBag.
+
+  Ltac insertOne :=
+    insertion CreateTerm EarlyIndex LastIndex
+              makeClause_dep EarlyIndex_dep LastIndex_dep.
